Practico 6.

TP6/predecesor.hs
@@ -1,0 +1,18 @@
+module Predecesor where
+
+import qualified Prelude
+
+data Nat =
+   O
+ | S Nat
+
+type Sig a =
+  a
+  -- singleton inductive, whose constructor was exist
+  
+predspec :: Nat -> Nat
+predspec n =
+  case n of {
+   O -> O;
+   S n0 -> n0}
+
