TP6/predecesor.ml
@@ -1,0 +1,14 @@
+type nat =
+| O
+| S of nat
+
+type 'a sig0 =
+  'a
+  (* singleton inductive, whose constructor was exist *)
+
+(** val predspec : nat -> nat **)
+
+let predspec = function
+| O -> O
+| S n0 -> n0
+
