TP6/practica6.v
@@ -1,0 +1,61 @@
+Section Ejercicio1.
+
+(* 1.1 *)
+Lemma predspec : forall n : nat,
+  {m : nat | n = 0 /\ m = 0 \/ n = S m}.
+Proof.
+  intro.
+  destruct n;
+  [ exists 0; left; split
+  | exists n; right
+  ]; reflexivity.
+Qed.
+
+End Ejercicio1.
+
+(* 1.2 *)
+Extraction Language Haskell.
+Extraction "predecesor" predspec.
+
+Section Ejercicio3.
+
+(* 3.1 *)
+Definition Value := bool.
+
+Inductive BoolExpr : Set :=
+| bbool : bool -> BoolExpr
+| or : BoolExpr -> BoolExpr -> BoolExpr
+| bnot : BoolExpr -> BoolExpr.
+
+Inductive BEval : BoolExpr -> Value -> Prop :=
+| ebool : forall b : bool, BEval (bbool b) (b:Value)
+| eorl : forall e1 e2 : BoolExpr, BEval e1 true -> BEval (or e1 e2) true
+| eorr : forall e1 e2 : BoolExpr, BEval e2 true -> BEval (or e1 e2) true
+| eorrl : forall e1 e2 : BoolExpr,
+BEval e1 false -> BEval e2 false -> BEval (or e1 e2) false
+| enott : forall e : BoolExpr, BEval e true -> BEval (bnot e) false
+| enotf : forall e : BoolExpr, BEval e false -> BEval (bnot e) true.
+
+Fixpoint beval (e : BoolExpr) : Value :=
+  match e with
+    | bbool b => b
+    | or e1 e2 =>
+    match beval e1, beval e2 with
+      | false, false => false
+      | _, _ => true
+    end
+    | bnot e1 => if beval e1 then false else true
+  end.
+
+Fixpoint sbeval (e : BoolExpr) : Value :=
+  match e with
+    | bbool b => b
+    | or e1 e2 =>
+    match sbeval e1 with
+      | true => true
+      | _ => sbeval e2
+    end
+    | bnot e1 => if sbeval e1 then false else true
+  end.
+
+End Ejercicio3.
